Migrate Interval CallString K1/K2 to declared globals

src/Examples/Interval/CallString/Example_Interval_DG_CallString_K2.thy
@@ -92,23 +92,23 @@ lemma callee_exit_g_f10_2: "(FunctionResult ''g'', [Statement 2, Statement 6]) \
 section \<open>Abstract transport of the routed solution\<close>
 
 lemma dg_tree_st_commute_frame_read_2:
-  "dg_tree_st_commute env
+  "dg_tree_st_commute_for nest_gs env
      (QueryG (Seed2 v ctx) (\<lambda>s. Answer (DG (globs s) bot)))
      (QueryG (Seed2 v ctx) (\<lambda>s. Answer (DG (globs s) bot)))"
-  by (simp add: dg_tree_st_commute_def fun_of_dg_st_simps fun_of_exec_dg_st_bot o_def
+  by (simp add: dg_tree_st_commute_for_def fun_of_dg_st_for_simps fun_of_exec_dg_st_for_bot o_def
                 dep_aux_def bot_fun_def)
 
 lemma dg_tree_st_commute_routed_cmb_2:
-  "dg_tree_st_commute env (routed_cmb Spoly Global2 (cs_route 2) ctx ca cc ex)
+  "dg_tree_st_commute_for nest_gs env (routed_cmb Spoly Global2 (cs_route 2) ctx ca cc ex)
                           (routed_cmb Sabs Global2 (cs_route 2) ctx ca cc ex)"
   unfolding routed_cmb_def Let_def
   by (cases ca)
-     (simp_all add: dg_tree_st_commute_def fun_of_dg_st_simps fun_of_exec_dg_st_bot o_def
+     (simp_all add: dg_tree_st_commute_for_def fun_of_dg_st_for_simps fun_of_exec_dg_st_for_bot o_def
                     cs_route_def dgs_combine_fst_commute_gen dgs_combine_snd_commute_gen
                     dep_aux_def bot_fun_def fun_upd_apply fun_eq_iff)
 
 lemma dg_tree_st_commute_routed_enter_pub_2:
-  "dg_tree_st_commute env
+  "dg_tree_st_commute_for nest_gs env
      (with_call a (\<lambda>dst fs as. do {
         entry_state \<leftarrow> read_local (v, ctx);
         globals_state \<leftarrow> read_global Global2;
@@ -126,12 +126,12 @@ lemma dg_tree_st_commute_routed_enter_pub_2:
         answer_local bot
       }))"
   by (cases a)
-     (simp add: dg_tree_st_commute_def fun_of_dg_st_simps fun_of_exec_dg_st_bot o_def
+     (simp add: dg_tree_st_commute_for_def fun_of_dg_st_for_simps fun_of_exec_dg_st_for_bot o_def
                 cs_route_def dgs_enter_fst_commute_gen dgs_enter_snd_commute_gen
                 dep_aux_def bot_fun_def fun_upd_apply fun_eq_iff)
 
 lemma hextra_commute_routed_2:
-  "list_all2 (dg_tree_st_commute env)
+  "list_all2 (dg_tree_st_commute_for nest_gs env)
      (routed_extra nest_cfg Spoly Seed2 Global2 (cs_route 2) ctx w)
      (routed_extra nest_cfg Sabs Seed2 Global2 (cs_route 2) ctx w)"
   unfolding routed_extra_def Let_def
@@ -158,8 +158,8 @@ theorem nest_2_pp_abs:
   "part_post_solution
      (side_cfg_T_eff_keyed_seed_dg intra_predecessor_list (\<lambda>_. Global2) (cs_route 2)
         (routed_cmb Sabs Global2) (routed_extra nest_cfg Sabs Seed2 Global2) nest_cfg Sabs
-        (fun_of_exec_dg_st (bot::ivl exec_dg_st)) (fun_of_exec_dg_st cinit_ivl_st) (fun_of_exec_dg_st (restrict_global_resolved_q cinit_ivl_st)))
-     (cfg_exit nest_cfg, []) (fun_of_dg_st \<circ> snd nest_2_sol) (fst nest_2_sol)"
+        (fun_of_exec_dg_st_for nest_gs (bot::ivl exec_dg_st)) (fun_of_exec_dg_st_for nest_gs cinit_ivl_st) (fun_of_exec_dg_st_for nest_gs (restrict_global_resolved_q cinit_ivl_st)))
+     (cfg_exit nest_cfg, []) (fun_of_dg_st_for nest_gs \<circ> snd nest_2_sol) (fst nest_2_sol)"
 proof -
   have pp': "part_post_solution
        (side_cfg_T_eff_keyed_seed_dg intra_predecessor_list (\<lambda>_. Global2) (cs_route 2)
@@ -168,12 +168,12 @@ proof -
        (cfg_exit nest_cfg, []) (snd nest_2_sol) (fst nest_2_sol)"
     using nest_2_pp_st unfolding nest_2_eqs_def by simp
   have ivl_Hstep_2:
-    "map_prod fun_of_exec_dg_st fun_of_exec_dg_st (dg_spec_step Spoly a d g') =
-       dg_spec_step Sabs a (fun_of_exec_dg_st d) (fun_of_exec_dg_st g')" for a d g'
+    "map_prod (fun_of_exec_dg_st_for nest_gs) (fun_of_exec_dg_st_for nest_gs) (dg_spec_step Spoly a d g') =
+       dg_spec_step Sabs a (fun_of_exec_dg_st_for nest_gs d) (fun_of_exec_dg_st_for nest_gs g')" for a d g'
     unfolding Spoly_def by (rule ivl_Hstep)
   show ?thesis
-    by (rule part_post_solution_seed_dg_st_to_abs
-          [where pred_sel = intra_predecessor_list and gkey = "\<lambda>_. Global2"
+    by (rule part_post_solution_seed_dg_st_to_abs_for
+          [where gs = nest_gs and pred_sel = intra_predecessor_list and gkey = "\<lambda>_. Global2"
              and route_st = "cs_route 2" and route_abs = "cs_route 2"
              and cmb_st = "routed_cmb Spoly Global2" and cmb_abs = "routed_cmb Sabs Global2"
              and extra_st = "routed_extra nest_cfg Spoly Seed2 Global2"
@@ -185,12 +185,12 @@ qed
 section \<open>Activation-indexed collecting soundness for the 2-call-string-routed solution\<close>
 
 abbreviation sigma_2 :: "pp \<times> cfg_node list + gk_2 \<Rightarrow> (ivl abs_state, ivl abs_state) dg_state" where
-  "sigma_2 \<equiv> fun_of_dg_st \<circ> snd nest_2_sol"
+  "sigma_2 \<equiv> fun_of_dg_st_for nest_gs \<circ> snd nest_2_sol"
 
 abbreviation gen_2_abs :: "(pp \<times> cfg_node list, gk_2, (ivl abs_state, ivl abs_state) dg_state) eqsT" where
   "gen_2_abs \<equiv> side_cfg_T_eff_keyed_seed_dg intra_predecessor_list (\<lambda>_. Global2) (cs_route 2)
        (routed_cmb Sabs Global2) (routed_extra nest_cfg Sabs Seed2 Global2) nest_cfg Sabs
-       (fun_of_exec_dg_st (bot::ivl exec_dg_st)) (fun_of_exec_dg_st cinit_ivl_st) (fun_of_exec_dg_st (restrict_global_resolved_q cinit_ivl_st))"
+       (fun_of_exec_dg_st_for nest_gs (bot::ivl exec_dg_st)) (fun_of_exec_dg_st_for nest_gs cinit_ivl_st) (fun_of_exec_dg_st_for nest_gs (restrict_global_resolved_q cinit_ivl_st))"
 
 lemma pp_eq_bound_2:
   "(v, ctx) \<in> fst nest_2_sol
@@ -225,9 +225,9 @@ lemma ivl_ctx_sg_2_uncovered_empty:
 
 lemma entry_locals_ge_s0d_2:
   assumes cov: "(cfg_entry nest_cfg, []) \<in> fst nest_2_sol"
-  shows "fun_of_exec_dg_st cinit_ivl_st \<le> locals (sigma_2 (Inl (cfg_entry nest_cfg, [])))"
+  shows "fun_of_exec_dg_st_for nest_gs cinit_ivl_st \<le> locals (sigma_2 (Inl (cfg_entry nest_cfg, [])))"
 proof -
-  have "fun_of_exec_dg_st cinit_ivl_st
+  have "fun_of_exec_dg_st_for nest_gs cinit_ivl_st
           \<le> locals (eq gen_2_abs (cfg_entry nest_cfg, []) sigma_2)"
     by (simp add: eq_side_cfg_T_eff_keyed_seed_dg)
        (rule order_trans[OF _ side_acc_dg_ge_2], simp add: le_supI2)
@@ -236,9 +236,9 @@ proof -
   finally show ?thesis .
 qed
 
-interpretation nest_2_dg: dg_ctx_activation Sabs is_global nest_cfg Global2 "cs_route 2"
+interpretation nest_2_dg: dg_ctx_activation Sabs nest_gs nest_cfg Global2 "cs_route 2"
     "routed_cmb Sabs Global2" "routed_extra nest_cfg Sabs Seed2 Global2"
-    "fun_of_exec_dg_st (bot::ivl exec_dg_st)" "fun_of_exec_dg_st cinit_ivl_st" "fun_of_exec_dg_st (restrict_global_resolved_q cinit_ivl_st)"
+    "fun_of_exec_dg_st_for nest_gs (bot::ivl exec_dg_st)" "fun_of_exec_dg_st_for nest_gs cinit_ivl_st" "fun_of_exec_dg_st_for nest_gs (restrict_global_resolved_q cinit_ivl_st)"
     sigma_2 "fst nest_2_sol" "(cfg_exit nest_cfg, [])" ivl_ctx_sg_2
 proof unfold_locales
   show "finite (intra nest_cfg)" by (rule nest_finE)
@@ -246,8 +246,8 @@ next
   show "part_post_solution
           (side_cfg_T_eff_keyed_seed_dg intra_predecessor_list (\<lambda>_. Global2) (cs_route 2)
              (routed_cmb Sabs Global2) (routed_extra nest_cfg Sabs Seed2 Global2) nest_cfg Sabs
-             (fun_of_exec_dg_st (bot::ivl exec_dg_st)) (fun_of_exec_dg_st cinit_ivl_st)
-             (fun_of_exec_dg_st (restrict_global_resolved_q cinit_ivl_st)))
+             (fun_of_exec_dg_st_for nest_gs (bot::ivl exec_dg_st)) (fun_of_exec_dg_st_for nest_gs cinit_ivl_st)
+             (fun_of_exec_dg_st_for nest_gs (restrict_global_resolved_q cinit_ivl_st)))
           (cfg_exit nest_cfg, []) sigma_2 (fst nest_2_sol)"
     by (rule nest_2_pp_abs)
 next
@@ -270,8 +270,8 @@ text \<open>Unlike \<open>k = 1\<close>, \<open>CallFwd\<close>'s \<open>Stateme
   is covered at two distinct one-element contexts, and \<open>take 2\<close> keeps them apart after
   routing, so each needs its own coverage witness.\<close>
 
-interpretation nest_2_routed: routed_context Sabs is_global nest_cfg Global2 "cs_route 2"
-    "fun_of_exec_dg_st (bot::ivl exec_dg_st)" "fun_of_exec_dg_st cinit_ivl_st" "fun_of_exec_dg_st (restrict_global_resolved_q cinit_ivl_st)"
+interpretation nest_2_routed: routed_context Sabs nest_gs nest_cfg Global2 "cs_route 2"
+    "fun_of_exec_dg_st_for nest_gs (bot::ivl exec_dg_st)" "fun_of_exec_dg_st_for nest_gs cinit_ivl_st" "fun_of_exec_dg_st_for nest_gs (restrict_global_resolved_q cinit_ivl_st)"
     sigma_2 "fst nest_2_sol" "(cfg_exit nest_cfg, [])" ivl_ctx_sg_2
     Seed2 "cs_enterc 2"
 proof (unfold_locales, goal_cases FinC SeedKey RouteAgree CallFwd CombFwd EnterAgree)
@@ -335,33 +335,33 @@ qed
 lemma ivl_ctx_sg_2_seed:
   assumes "(u, CallEdge dst xs es, FunctionEntry p, cont) \<in> calls nest_cfg"
     and "s \<in> \<lbrakk>ivl_ctx_sg_2 (Inl (u, ctx))\<rbrakk>"
-  shows "call_enter is_global (CallEdge dst xs es) s
+  shows "call_enter nest_gs (CallEdge dst xs es) s
            \<in> \<lbrakk>ivl_ctx_sg_2 (Inl (FunctionEntry p,
-                 cs_enterc 2 u ctx (call_enter is_global (CallEdge dst xs es) s)))\<rbrakk>"
+                 cs_enterc 2 u ctx (call_enter nest_gs (CallEdge dst xs es) s)))\<rbrakk>"
   by (rule nest_2_routed.routed_context_call[OF assms])
 
 lemma ivl_ctx_sg_2_comb:
   assumes "(cl, CallEdge dst pars args, FunctionEntry p, v) \<in> calls nest_cfg"
     and "s \<in> \<lbrakk>ivl_ctx_sg_2 (Inl (cl, c1))\<rbrakk>"
     and "t \<in> \<lbrakk>ivl_ctx_sg_2 (Inl (FunctionResult p, cs_enterc 2 cl c1 es))\<rbrakk>"
-    and "call_enter_store is_global nest_cfg cl s es"
-  shows "combine_collect is_global dst s t \<in> \<lbrakk>ivl_ctx_sg_2 (Inl (v, c1))\<rbrakk>"
+    and "call_enter_store nest_gs nest_cfg cl s es"
+  shows "combine_collect nest_gs dst s t \<in> \<lbrakk>ivl_ctx_sg_2 (Inl (v, c1))\<rbrakk>"
   by (rule nest_2_routed.routed_context_comb[OF assms])
 
 section \<open>The headline theorem: 2-call-string activation collecting soundness\<close>
 
-lemma cinit_le_cinit_ivl_st_2: "cinit_stores is_global \<subseteq> \<lbrakk>fun_of_exec_dg_st cinit_ivl_st\<rbrakk>"
-  by (auto simp: cinit_stores_def gamma_state_def fun_of_st_cinit_ivl_st)
+lemma cinit_le_cinit_ivl_st_2: "cinit_stores nest_gs \<subseteq> \<lbrakk>fun_of_exec_dg_st_for nest_gs cinit_ivl_st\<rbrakk>"
+  by (auto simp: cinit_stores_def gamma_state_def fun_of_exec_dg_st_for_def fun_of_st_cinit_ivl_st_for)
 
 theorem nest_2_activation_collect_sound:
-  "activation_collect is_global (cs_enterc 2) [] nest_cfg (cinit_stores is_global) v ctx
+  "activation_collect nest_gs (cs_enterc 2) [] nest_cfg (cinit_stores nest_gs) v ctx
      \<subseteq> \<lbrakk>ivl_ctx_sg_2 (Inl (v, ctx))\<rbrakk>"
 proof (rule activation_collect_sound[where sg = ivl_ctx_sg_2 and enterc = "cs_enterc 2"
-        and seedc = "[]" and S = "cinit_stores is_global" and g = nest_cfg and gs = is_global])
+        and seedc = "[]" and S = "cinit_stores nest_gs" and g = nest_cfg and gs = nest_gs])
   \<comment> \<open>ENTRY_G\<close>
-  fix s assume "s \<in> cinit_stores is_global"
-  hence "s \<in> \<lbrakk>fun_of_exec_dg_st cinit_ivl_st\<rbrakk>" using cinit_le_cinit_ivl_st_2 by blast
-  also have "\<lbrakk>fun_of_exec_dg_st cinit_ivl_st\<rbrakk>
+  fix s assume "s \<in> cinit_stores nest_gs"
+  hence "s \<in> \<lbrakk>fun_of_exec_dg_st_for nest_gs cinit_ivl_st\<rbrakk>" using cinit_le_cinit_ivl_st_2 by blast
+  also have "\<lbrakk>fun_of_exec_dg_st_for nest_gs cinit_ivl_st\<rbrakk>
         \<subseteq> \<lbrakk>locals (sigma_2 (Inl (cfg_entry nest_cfg, [])))\<rbrakk>"
     by (rule gamma_state_mono[OF entry_locals_ge_s0d_2[OF entry_covered_2]])
   also have "\<dots> \<subseteq> \<lbrakk>ivl_ctx_sg_2 (Inl (cfg_entry nest_cfg, []))\<rbrakk>"
@@ -378,9 +378,9 @@ next
   show "\<And>u dst pars args p cont c s.
         (u, CallEdge dst pars args, FunctionEntry p, cont) \<in> calls nest_cfg
         \<Longrightarrow> s \<in> \<lbrakk>ivl_ctx_sg_2 (Inl (u, c))\<rbrakk>
-        \<Longrightarrow> call_enter is_global (CallEdge dst pars args) s
+        \<Longrightarrow> call_enter nest_gs (CallEdge dst pars args) s
              \<in> \<lbrakk>ivl_ctx_sg_2 (Inl (FunctionEntry p,
-                    cs_enterc 2 u c (call_enter is_global (CallEdge dst pars args) s)))\<rbrakk>"
+                    cs_enterc 2 u c (call_enter nest_gs (CallEdge dst pars args) s)))\<rbrakk>"
     by (rule ivl_ctx_sg_2_seed)
 next
   \<comment> \<open>COMB --- return combine at the caller's own truncated context.\<close>
@@ -388,8 +388,8 @@ next
         (cl, CallEdge dst pars args, FunctionEntry p, cont) \<in> calls nest_cfg
         \<Longrightarrow> s \<in> \<lbrakk>ivl_ctx_sg_2 (Inl (cl, c1))\<rbrakk>
         \<Longrightarrow> t \<in> \<lbrakk>ivl_ctx_sg_2 (Inl (FunctionResult p, cs_enterc 2 cl c1 es))\<rbrakk>
-        \<Longrightarrow> call_enter_store is_global nest_cfg cl s es
-        \<Longrightarrow> combine_collect is_global dst s t \<in> \<lbrakk>ivl_ctx_sg_2 (Inl (cont, c1))\<rbrakk>"
+        \<Longrightarrow> call_enter_store nest_gs nest_cfg cl s es
+        \<Longrightarrow> combine_collect nest_gs dst s t \<in> \<lbrakk>ivl_ctx_sg_2 (Inl (cont, c1))\<rbrakk>"
     by (rule ivl_ctx_sg_2_comb)
 qed
 
@@ -410,10 +410,10 @@ definition nest_2_graph_config ::
           nest_cfg p)),
       globals_to_show = [],
       show_local = (\<lambda>p ctx vars d. map (\<lambda>x.
-        x @ ''='' @ string_of_ivl (lookup_exec_dg_st d x)) vars),
+        x @ ''='' @ string_of_ivl (nest_lookup_exec_dg_st d x)) vars),
       format_return = (\<lambda>p ctx ret d.
-        if lookup_exec_dg_st d ret = ivl_top then []
-        else [''ret='' @ string_of_ivl (lookup_exec_dg_st d ret)]),
+        if nest_lookup_exec_dg_st d ret = ivl_top then []
+        else [''ret='' @ string_of_ivl (nest_lookup_exec_dg_st d ret)]),
       show_global = (\<lambda>k vars s. [''(none)'']),
       show_global_key = (\<lambda>k. case k of Global2 \<Rightarrow> ''Global'' | Seed2 p ctx \<Rightarrow> ''Seed''),
       is_shared_global = (\<lambda>k. case k of Global2 \<Rightarrow> True | Seed2 _ _ \<Rightarrow> False),
@@ -467,5 +467,4 @@ lemma nest_2_dot_nonempty: "String.explode nest_2_dot \<noteq> []" by eval
 ML_val \<open>writeln (@{code nest_2_dot})\<close>
 
 end
-
 
